\documentclass[11pt,letterpaper]{article}
\usepackage[utf8]{inputenc}
\usepackage{amsmath}
\usepackage{amsfonts}
\usepackage{xcolor}
\usepackage{multicol}
\usepackage{rotating}
\usepackage{amssymb}
\usepackage{graphicx}
\usepackage[left=1cm,right=1cm,top=2cm,bottom=2cm]{geometry}
\makeatletter
\def\tagform@#1{\maketag@@@{[\ignorespaces#1\unskip\@@italiccorr]}}
\makeatother
\newcommand{\fstep}[1]{$$\color{red}{\Downarrow\mbox{Step #1}\Downarrow}$$}
\begin{document}
\begin{sidewaysfigure}
\begin{multicols}{2}
\setcounter{equation}{-1}
\begin{equation}
ax^2+bx+c=0
\end{equation}
\fstep{1}
\begin{equation}
ax^2+bx=-c
\end{equation}
\fstep{2}
\begin{equation}
x^2+{b\over a}x=-{c\over a}
\end{equation}
\fstep{3}
\begin{equation}
x^2+{b\over a}x+\left({b\over 2a}\right)^2=-{c\over a}+\left({b\over 2a}\right)^2
\end{equation}
\fstep{4}
\begin{equation}
\left(x+{b\over 2a}\right)^2=-{c\over a}+\left({b\over 2a}\right)^2
\end{equation}
\fstep{5}
\begin{equation}
\left(x+{b\over 2a}\right)^2=-{c\over a}+{b^2\over 4a^2}
\end{equation}
\fstep{6}
\begin{equation}
\left(x+{b\over 2a}\right)^2={b^2\over 4a^2}-{c\over a}
\end{equation}
\fstep{7}
\begin{equation}
\left(x+{b\over 2a}\right)^2={b^2\over 4a^2}-{4c\over 4a}
\end{equation}
\fstep{8}
\begin{equation}
\left(x+{b\over 2a}\right)^2={b^2\over 4a^2}-{4ac\over 4a^2}
\end{equation}
\fstep{9}
\begin{equation}
\left(x+{b\over 2a}\right)^2={b^2-4ac\over 4a^2}
\end{equation}
\fstep{10}
\begin{equation}
\sqrt{\left(x+{b\over 2a}\right)^2}=\pm\sqrt{{b^2-4ac\over 4a^2}}
\end{equation}
\fstep{11}
\begin{equation}
x+{b\over 2a}=\pm\sqrt{{b^2-4ac\over 4a^2}}
\end{equation}
\fstep{12}
\begin{equation}
x=-{b\over 2a}\pm\sqrt{{b^2-4ac\over 4a^2}}
\end{equation}
\fstep{13}
\begin{equation}
x=-{b\over 2a}\pm{\sqrt{b^2-4ac}\over 2a}
\end{equation}
\fstep{14}
\begin{equation}
x={-b\pm\sqrt{b^2-4ac}\over 2a}
\end{equation}
\end{multicols}
\end{sidewaysfigure}
\end{document}